theories/metaprogramming/pull_transport_test_2.v
@@ -1,0 +1,70 @@
+
+
+(*
+An idea is, can I just recalculate the equality for the cast being on the other side?
+ *)
+
+Definition cast {x y : Type} (p : x = y) : x -> y.
+Proof.
+  intros.
+  subst.
+  assumption.
+Defined.
+
+Axiom uip : forall T (t1 t2 : T) (p1 p2 : t1 = t2), p1 = p2.
+
+Theorem pull_through_1
+        (I : Type)
+        (P Q : I -> Type)
+        (f : forall {i}, P i -> Q i)
+        (i1 i2 : I)
+        (pin : P i1 = P i2)
+        (*pout : Q i1 = Q i2*)
+        (realp : i1 = i2)
+        (input : P i1)
+  : f (cast pin input) = cast (f_equal Q realp) (f input).
+Proof.
+  subst.
+  (*rewrite (uip _ _ _ pout eq_refl).*)
+  rewrite (uip _ _ _ pin eq_refl).
+  reflexivity.
+Qed.
+
+(*
+The idea is that I can just recompute realp with solve_all whenever I want to use this rewrite.
+*)
+
+Definition transport {T : Type} (P : T -> Type) {t1 t2 : T} (p : t1 = t2) (a : P t1) : P t2.
+  subst.
+  apply a.
+Defined.
+
+Theorem pull_through_1
+        (I : Type)
+        (P Q : I -> Type)
+        (f : forall {i}, P i -> Q i)
+        (i1 i2 : I)
+        (p : i1 = i2)
+        (input : P i1)
+  : f (transport P p input) = transport Q p (f input).
+Proof.
+  refine match p with
+         | eq_refl => _
+         end.
+  reflexivity.
+Qed.
+
+Axiom Fam : nat -> Type.
+Axiom f1 : forall {n}, Fam (10 + n) -> Fam (n - 20).
+
+(*
+Theorem test_1
+        (p : 15 = 25)
+        (input : Fam 15)
+  : f1 (transport Fam p input) = transport Fam p (f1 input).
+Proof.
+  Check (transport Fam p input).
+  Check (f1 (transport _ p input)).
+  Fail rewrite pull_through_1.
+  rewrite 
+*)
