theories/metaprogramming/substitution2.v
@@ -1,0 +1,299 @@
+Require Import String.
+Require Import qterm.
+Require Import lambdaFacts.
+Require Import lambdaSolve.
+Require Import FunctionalExtensionality.
+Require Import Coq.Logic.PropExtensionality.
+
+(*
+In this version, I'm going to try using a single cast going directly between types
+with no index.
+I'm trying the approach pull_through_1 from pull_transport_through_2.v
+The idea is that it will use solve_all to prove the indices equal.
+*)
+
+Module S.
+  Definition nil := <Nil>.
+  Definition cons := <fun ctx => fun lvl => fun ty => Cons ctx lvl ty>.
+
+  Definition zero := <fun env => proj2 env>.
+  Definition succ := <fun x => fun env => x (proj1 env)>.
+
+  Definition level (n : nat) : QTerm := const n.
+
+  Definition pi := <fun x => fun y => fun env => Pi (x env) (fun a => y (env , a))>.
+  Definition U : QTerm := <fun env => U>.
+  Definition Empty := <fun env => Empty>.
+  Definition Bool := <fun env => Bool>.
+  Definition Lift := <fun T => fun env => Lift (T env)>.
+
+  Definition var_to_term := <fun x => x>.
+  Definition lambda := <fun t => fun env => fun a => t (env , a)>.
+  Definition app := <fun t1 => fun t2 => fun env => (t1 env) (t2 env)>.
+  Definition true := <fun env => fun p => proj1 p>.
+  Definition false := <fun env => fun p => proj2 p>.
+  Definition ifexpr := <fun cond => fun t1 => fun t2 => fun env => (cond env) (t1 env, t2 env)>.
+
+  Definition weaken := <fun t => fun env => t (proj1 env)>.
+  Definition subLast := <fun t => fun toSub => fun env => t (env , toSub env)>.
+
+  (* Shallow substitutions *)
+  Definition idSub := <fun env => env>. (* : Sub ctx ctx *)
+  Definition weaken1Ren := <fun env => proj1 env>. (* : Sub ctx (ctx, T) *)
+  (* liftSub : Sub ctx1 ctx2 -> Sub (cons ctx1 lvl T) (cons ctx2 lvl (subTerm sub T)) *)
+  Definition liftSub := <fun sub => fun env => (sub (proj1 env), proj2 env)>.
+  (* subTerm : (sub : Sub ctx1 ctx2) -> Term ctx1 T -> Term ctx2 (subTerm sub T) *)
+  (* extendSub : Sub ctx1 ctx2 -> Term ctx1 T -> Sub (ctx1, T) ctx2 *)
+  Definition extendSub := <fun sub => fun t => fun env => (sub env, t (sub env))>.
+  Definition subTerm := <fun sub => fun t => fun env => t (sub env)>.
+
+  Ltac unfold_all := unfold nil, cons, zero, succ, pi, U, Bool, Empty, var_to_term, lambda,
+      app, weaken, subLast, level, true, false, ifexpr, Lift,
+      idSub, weaken1Ren, liftSub, subTerm in *.
+End S.
+
+(* The deeper shallow embedding *)
+
+Inductive Var : QTerm -> nat -> QTerm -> QTerm -> Type :=
+| zero : forall {ctx T lvl}, Var <`S.cons `ctx {const lvl} `T> lvl <`S.weaken `T> S.zero
+| succ : forall {ctx A T s lvl1 lvl2}, Var ctx lvl1 A s
+                              -> Var <`S.cons `ctx `lvl2 `T> lvl1 <`S.weaken `A> <`S.succ `s>.
+
+Inductive Typed : (*context*) QTerm -> (*level*) nat -> (*Type*) QTerm -> (*Term*) QTerm -> Type :=
+| lambda : forall {ctx A B s lvl},
+    (*Typed ctx (S lvl) <`U(*{const lvl}*)> <`pi `A `B> ->*)
+    Typed <`S.cons `ctx {const lvl} `A> lvl B s -> Typed ctx lvl <`S.pi `A `B> <`S.lambda `s>
+(*
+| app : forall ctx A B s1 s2 lvl, Typed ctx lvl <`pi `A `B> s1 -> Typed ctx lvl A s2
+                                 -> Typed ctx lvl <`subLast `B `s2> <`app `s1 `s2>*)
+| var : forall {ctx T t lvl}, Var ctx lvl T t -> Typed ctx lvl T t
+| true : forall {ctx}, Typed ctx 0 S.Bool S.true
+| false : forall {ctx}, Typed ctx 0 S.Bool S.false
+(*
+| if : forall ctx T cond t1 t2 lvl,
+    Typed ctx lvl Bool cond ->
+    Typed ctx lvl <`subLast `T `true> t1 ->
+    Typed ctx lvl <`subLast `T `false> t2 ->
+    Typed ctx lvl <`subLast `T `cond> <`ifexpr `cond `t1 `t2>
+| Empty : forall ctx, Typed ctx 1 <`U(*{const 0}*)> Empty
+| Bool : forall ctx, Typed ctx 1 <`U(*{const 0}*)> Bool
+| pi : forall ctx A B lvl,
+    Typed ctx (S lvl) <`U(*{const lvl}*)> A
+    (* TODO: is S lvl correct below? *)
+    -> Typed <`cons `ctx {const lvl} `A> (S lvl) <`U(*{const lvl}*)> B -> Typed ctx (S lvl) <`U(*{const lvl}*)> <`pi `A `B>
+| U : forall ctx lvl, Typed ctx (S (S lvl)) <`U(*{const (S lvl)}*)> <`U(*{const lvl}*)>
+| Lift : forall ctx lvl T, Typed ctx (S lvl) <`U> T -> Typed ctx (S (S lvl)) <`U> <`Lift `T>
+| lift : forall ctx lvl T t, Typed ctx lvl T t -> Typed ctx (S lvl) <`Lift `T> t
+| lower : forall ctx lvl T t, Typed ctx (S lvl) <`Lift `T> t -> Typed ctx lvl T t
+*)
+.
+
+Ltac solve_no_unfold := repeat (lambda_solve ; repeat neutral_inj_case ;lambda_solve
+                  ; repeat fast_neutral_unequal_case). 
+
+Ltac solve_all := repeat (try S.unfold_all ;
+                          try lambda_solve ;
+                          (repeat neutral_inj_case ; lambda_solve);
+                          (repeat fast_neutral_unequal_case);
+                          (repeat simple_pattern_case);
+                          (repeat pair_pattern_case; subst);
+                          hide_evars;
+                          rewrite <- ?eta, <- ?SP;
+                          sort_lifts;
+                          unhide_evars).
+
+Definition cast {x y : Type} {p : x = y} : x -> y.
+Proof.
+  intros.
+  subst.
+  assumption.
+Defined.
+
+Axiom uip : forall T (t1 t2 : T) (p1 p2 : t1 = t2), p1 = p2.
+
+Theorem remove_cast
+        (T : Type)
+        (p : T = T)
+        (input : T)
+        : @cast _ _ p input = input.
+Proof.
+  rewrite (uip _ _ _ p eq_refl).
+  reflexivity.
+Qed.
+
+Definition Ren (sub ctx1 ctx2 : QTerm) : Type :=
+  forall {lvl T t}, Var ctx1 lvl T t -> Var ctx2 lvl <`S.subTerm `sub `T> <`S.subTerm `sub `t>.
+
+Definition idRen {ctx} : Ren S.idSub ctx ctx.
+  refine (fun lvl T t x => cast x); solve_all.
+Defined.
+
+Definition liftRen {ctx1 ctx2 lvl T sub} (ren : Ren sub ctx1 ctx2)
+  : Ren <`S.liftSub `sub> <`S.cons `ctx1 `lvl `T> <`S.cons `ctx2 `lvl (`S.subTerm `sub `T)>.
+intros lvl2 T2 t2 x.
+remember <`S.cons `ctx1 `lvl `T> as ctx in x.
+generalize dependent Heqctx.
+refine (match x with
+        | zero  => fun _ => cast zero
+        | succ x' => fun _ => cast (succ (ren _ _ _ (cast x')))
+        end); solve_all.
+Defined.
+
+Definition weaken1Ren {ctx lvl T}
+  : Ren S.weaken1Ren ctx <`S.cons `ctx `lvl `T>.
+unfold Ren.
+intros lvl' T' t' x.
+refine (cast (succ x)); solve_all.
+Defined.
+(*
+So the above works. However, somewhere deep in a solve_all, it uses reflexivity to solve a goal
+like
+?x [x] (`t1 [x] x) = `t2 [x] (`t1 [x] x)
+where `t1 and `t2 are rocq "metavariables", and ?x is an evar.
+I'm not sure if this is correct, since the evar wasn't exactly "forced" to have the value `t2.
+*)
+
+Fixpoint renTerm {ctx1 ctx2 sub lvl T t} (ren : Ren sub ctx1 ctx2)
+           (prog : Typed ctx1 lvl T t) : Typed ctx2 lvl <`S.subTerm `sub `T> <`S.subTerm `sub `t>.
+generalize dependent ren.
+refine (match prog with
+        | lambda t => fun ren => cast (lambda (renTerm _ _ _ _ _ _ (liftRen ren) t))
+        | var x => fun ren => var (ren _ _ _ (cast x))
+        | true => fun _ => cast true
+        | false => fun _ => cast false
+        end ); solve_all.
+Defined.
+
+Definition run_ren_1_statement : Prop.
+  refine (renTerm (@idRen S.nil) true = cast true); solve_all.
+Defined.  
+Theorem run_ren_1 : run_ren_1_statement.
+Proof.
+  unfold run_ren_1_statement.
+  simpl.
+  Fail reflexivity.
+Abort.
+
+Check @cast.
+
+Theorem compose_cast
+        (A B C : Type)
+        (p1 : A = B)
+        (p2 : B = C)
+        (input : A)
+  : @cast _ _ p2 (@cast _ _ p1 input) = @cast _ _ (eq_trans p1 p2) input.
+Proof.
+  subst.
+  reflexivity.
+Qed.
+
+
+Definition run_ren_1_statement' : Prop.
+  refine (cast (renTerm (@idRen S.nil) true) = true); solve_all.
+Defined.
+Theorem run_ren_1' : run_ren_1_statement'.
+Proof.
+  unfold run_ren_1_statement'.
+  simpl.
+  rewrite compose_cast.
+  rewrite remove_cast.
+  reflexivity.
+Qed.
+
+(*
+Trying applying a renaming to a term.
+renaming = succ, starting with a context with 1 free variable
+term = \x0. x1
+should get renamed into \x0. x2
+*)
+
+(* TODO: solve_all should be able to infer the type, term, and level indices.
+ can I get rocq to allow me to leave those as evars? *)
+Definition prog1 : Typed <`S.cons `S.nil {const 0} `S.Bool> 0
+                         <`S.pi `S.Bool `S.Bool>
+                     <`S.lambda (`S.var_to_term (`S.succ `S.zero))>.
+refine (cast (lambda (var (succ zero)))); solve_all.
+Defined.
+
+Definition prog2 : Typed <`S.cons (`S.cons `S.nil {const 0} `S.Bool) {const 0} `S.Bool> 0
+                         <`S.pi `S.Bool `S.Bool>
+                     <`S.lambda (`S.var_to_term (`S.succ (`S.succ `S.zero)))>.
+refine (cast (lambda (var (succ (succ zero))))); solve_all.
+Defined.
+
+
+Axiom eq_cheat : forall {T} {x y : T}, x = y.
+Axiom replace_eq : forall T (x y : T) (p : x = y), p = eq_cheat.
+Import HiddenMark.
+Theorem compact_cast
+        (A B : Type)
+        (p : A = B)
+        (input : A)
+  : @cast _ _ p input
+    = ((Mark (@cast)) _ _ eq_cheat input).
+Proof.
+  rewrite (replace_eq _ _ _ p).
+  rewrite MarkIsJustId.
+  reflexivity.
+Qed.
+
+Ltac garbage_compact := repeat rewrite compact_cast;
+                        repeat rewrite MarkIsJustId.
+
+Theorem pull_cast_through
+        (I : Type)
+        (P Q : I -> Type)
+        (f : forall {i}, P i -> Q i)
+        (i1 i2 : I)
+        (pin : P i1 = P i2)
+        (realp : i1 = i2)
+        (input : P i1)
+  : f (@cast _ _ pin input) = @cast _ _ (f_equal Q realp) (f input).
+Proof.
+  subst.
+  rewrite (uip _ _ _ pin eq_refl).
+  reflexivity.
+Qed.
+
+Check pull_cast_through.
+Search sigT.
+
+Import SigTNotations.
+Check fst.
+Check @renTerm.
+Definition renTerm' {args : {ctx1 : QTerm & {ctx2 : QTerm & {sub : QTerm & {lvl : nat &                                              {T : QTerm & {t : QTerm & Ren sub ctx1 ctx2}}}}}}}
+           (prog : Typed (args .1) (args .2 .2 .2 .1) (args .2 .2 .2 .2 .1) (args .2 .2 .2 .2 .2 .1))
+  : Typed (args .2 .1) (args .2 .2 .2 .1) <`S.subTerm {args .2 .2 .1} {args .2 .2 .2 .2 .1}>
+      <`S.subTerm {args .2 .2 .1} {args .2 .2 .2 .2 .2 .1}> :=
+  @renTerm (args .1) (args .2 .1) (args .2 .2 .1) (args .2 .2 .2 .1) (args .2 .2 .2 .2 .1)
+           (args .2 .2 .2 .2 .2 .1) (args .2 .2 .2 .2 .2 .2) prog.
+
+Definition run_ren_2_statement : Prop.
+  refine (cast (renTerm' (_ ; (_ ; (_ ; (_ ; (_ ; (_ ; weaken1Ren)))))) prog1) = prog2); solve_all.
+Defined.
+
+
+Theorem run_ren_2 : run_ren_2_statement.
+Proof.
+  unfold run_ren_2_statement, prog1, prog2.
+  Check (@renTerm).
+  Check (fun ctx lvl ty tm => @renTerm ctx _ _ lvl ty tm weaken1Ren).
+  garbage_compact.
+  Check pull_cast_through.
+  match goal with
+  | |- context [?f (cast ?arg)] => idtac f
+  end.
+  rewrite (@pull_cast_through _ _ _
+               (fun i => @renTerm (fst (fst i)) _ _ (snd (fst i)) (fst (snd i)) (snd (snd i)) weaken1Ren)).
+(*                 (fun ctx lvl ty tm => @renTerm ctx _ _ lvl ty tm weaken1Ren)).*)
+  simpl.
+  garbage_compact.
+  repeat rewrite compose_cast.
+  unfold weaken1Ren.
+  garbage_compact.
+  Check @succ.
+  repeat rewrite (@push_transport_through_var _ _ _ _
+                                              (fun ctx lvl ty tm => @succ ctx ty _ tm lvl _)).
+  repeat rewrite compose_castVar.
+  rewrite (@push_transport_through_var_term _ _ _ _
+                                            (fun ctx lvl ty tm => @var ctx ty tm lvl)).
